examples/composite_game.v
@@ -17,7 +17,7 @@ Unset Printing Implicit Defensive.
 
 Section Game.
 
-Context `{!cryptisGS Σ, !heapGS Σ, !spawnG Σ, !crGS Σ, !tlsGS Σ, !nsl_dhGS Σ}.
+Context `{!cryptisGS Σ, !heapGS Σ, !spawnG Σ, !nsl_dhGS Σ}.
 Notation iProp := (iProp Σ).
 
 Implicit Types t : term.
@@ -27,6 +27,9 @@ Implicit Types skI skR : sign_key.
 Definition nslN := nroot.@"nsldh".
 Definition crN := nroot.@"cr".
 Definition tlsN := nroot.@"tls".
+
+Definition trivP : role → term → term → sign_key → sign_key → iProp :=
+  λ _ _ _ _ _, True%I.
 
 Definition loop : val := λ: "f",
   rec: "loop" <> := "f" #();; "loop" #().
@@ -111,8 +114,7 @@ Lemma wp_environment c (skI1 skR1 : aenc_key) (skI2 skR2 : sign_key) (psk : term
   channel c -∗
   nsl_dh_ctx -∗
   nsl_dh_pred nslN (λ _ _ _ _, True)%I -∗
-  cr_ctx crN -∗
-  cr_pred crN (λ _ _ _ _ _, True)%I -∗
+  cr_ctx crN trivP -∗
   tls_ctx tlsN -∗
   public skI1 -∗
   public skR1 -∗
@@ -121,7 +123,7 @@ Lemma wp_environment c (skI1 skR1 : aenc_key) (skI2 skR2 : sign_key) (psk : term
   minted psk -∗
   {{{ True }}} environment c skI1 skI2 skR1 skR2 psk {{{ RET #(); True }}}.
 Proof.
-iIntros "#? #? #? #? #? #? #? #? #? #? #? #? %Φ !> _ post".
+iIntros "#? #? #? #? #? #? #? #? #? #? #? %Φ !> _ post".
 rewrite /environment; wp_pures.
 wp_bind (send _ _); iApply wp_send => //; wp_pures.
 wp_bind (send _ _); iApply wp_send => //; wp_pures.
@@ -229,23 +231,18 @@ Lemma wp_game :
   cryptis_ctx ∗
   nsl_dh_ctx ∗
   nsl_dh_token ⊤ ∗
-  cr_token ⊤ ∗
-  tls_token ⊤ ∗
   seal_pred_token SIGN ⊤ ∗
   seal_pred_token SENC ⊤ ∗
   hash_pred_token ⊤ -∗
   WP game #() {{ v, ⌜v = NONEV ∨ v = SOMEV #true⌝ }}.
 Proof.
-iIntros "(#ctx & #nsl_ctx & nsl_tok & cr_tok & tls_tok &
-          sign_tok & senc_tok & hash_tok)".
+iIntros "(#ctx & #nsl_ctx & nsl_tok & sign_tok & senc_tok & hash_tok)".
 rewrite /game; wp_pures.
 iMod (nsl_dh_pred_set nslN (λ _ _ _ _, True)%I with "nsl_tok")
   as "(#nsl_pred & nsl_tok)"; first solve_ndisj.
-iMod (cr_alloc crN with "sign_tok") as "(#cr_ctx & sign_tok)"; first solve_ndisj.
-iMod (cr_pred_set crN (λ _ _ _ _ _, True)%I with "cr_tok")
-  as "(#cr_pred & cr_tok)"; first solve_ndisj.
-iMod (tls_ctx_alloc tlsN with "tls_tok senc_tok sign_tok hash_tok")
-  as "(#tls_ctx & tls_tok & senc_tok & sign_tok & hash_tok)"; try solve_ndisj.
+iMod (cr_alloc crN trivP with "sign_tok") as "(#cr_ctx & sign_tok)"; first solve_ndisj.
+iMod (tls_ctx_alloc tlsN with "senc_tok sign_tok hash_tok")
+  as "(#tls_ctx & senc_tok & sign_tok & hash_tok)"; try solve_ndisj.
 wp_apply wp_init_network => //. iIntros "%c #cP". wp_pures.
 wp_apply wp_mk_aenc_key => //. iIntros "%skI1 #? s_skI1 _".
 iMod (secret_public with "s_skI1") as "#?". wp_pures.
@@ -278,7 +275,7 @@ Qed.
 End Game.
 
 Definition F : gFunctors :=
-  #[heapΣ; spawnΣ; cryptisΣ; crΣ; tlsΣ; nsl_dhΣ].
+  #[heapΣ; spawnΣ; cryptisΣ; nsl_dhΣ].
 
 Lemma composite_secure σ₁ σ₂ (v : val) ts :
   rtc erased_step ([game #()], σ₁) (Val v :: ts, σ₂) →
@@ -289,8 +286,6 @@ apply (adequate_result NotStuck _ _ (λ v _, v = NONEV ∨ v = SOMEV #true)).
 apply: heap_adequacy.
 iIntros (?) "?".
 iMod (cryptisGS_alloc _) as (?) "(#ctx & aenc_tok & sign_tok & senc_tok & hash_tok)".
-iMod crGS_alloc as (?) "cr_tok".
-iMod tlsGS_alloc as (?) "tls_tok".
 iMod (nsl_dhGS_alloc with "aenc_tok") as (?) "(#nsl_ctx & nsl_tok & _)".
 { solve_ndisj. }
 by iApply (wp_game) => //; iFrame "∗ #".
